\documentclass{article}
\usepackage{mathtools}
\usepackage{amssymb}
\begin{document}

\begin{align*}
\frac{\partial^{2}L}{\partial w_{j}\partial w_{k}} &=  \frac{\partial L}{\partial w_{k}}(\sum_{i=1}^{N}\frac{e^{y_{i}(w^{T}x_{i}+b)}}{(1+e^{y_{i}(w^{T}x_{i}+b)})}\cdot x_{ij}y_{i}+2\lambda w_{j})\\
&= \sum_{i=1}^{N}\frac{x_{ij}y_{i}\cdot(1+e^{y_{i}(w^{T}x_{i}+b)})\cdot\frac{\partial L}{\partial w_{k}}(e^{y_{i}(w^{T}x_{i}+b)})-e^{y_{i}(w^{T}x_{i}+b)}\cdot\frac{\partial L}{\partial w_{k}}(1+e^{y_{i}(w^{T}x_{i}+b)})}{(1+e^{y_{i}(w^{T}x_{i}+b)})^{2}}\\
&= \sum_{i=1}^{N}\frac{x_{ij}y_{i}\cdot(1+e^{y_{i}(w^{T}x_{i}+b)})\cdot\frac{\partial L}{\partial w_{k}}(e^{y_{i}(w^{T}x_{i}+b)})-e^{y_{i}(w^{T}x_{i}+b)}\cdot\frac{\partial L}{\partial w_{k}}(e^{y_{i}(w^{T}x_{i}+b)})}{(1+e^{y_{i}(w^{T}x_{i}+b)})^{2}}\\
&= \sum_{i=1}^{N}\frac{x_{ij}y_{i}\cdot(1+e^{y_{i}(w^{T}x_{i}+b)}-e^{y_{i}(w^{T}x_{i}+b)})\cdot\frac{\partial L}{\partial w_{k}}(e^{y_{i}(w^{T}x_{i}+b)})}{(1+e^{y_{i}(w^{T}x_{i}+b)})^{2}}\\
&= \sum_{i=1}^{N}\frac{x_{ij}y_{i}\cdot \frac{\partial L}{\partial w_{k}}(e^{y_{i}(w^{T}x_{i}+b)})}{(1+e^{y_{i}(w^{T}x_{i}+b)})^{2}}\\
&= \sum_{i=1}^{N}\frac{x_{ij}y_{i}\cdot e^{y_{i}(w^{T}x_{i}+b)}x_{ik}y_{i}}{(1+e^{y_{i}(w^{T}x_{i}+b)})^{2}}\\
&= \sum_{i=1}^{N}\frac{x_{ij}x_{ik}y_{i}y_{i}\cdot e^{y_{i}(w^{T}x_{i}+b)}}{(1+e^{y_{i}(w^{T}x_{i}+b)})^{2}}\\
\end{align*}
Since \(y_i^2 = 1\), we simply rewrite this as
\begin{equation}
  \sum_{i=1}^{N}x_{ij}x_{ik}\cdot \frac{e^{y_{i}(w^{T}x_{i}+b)}}{(1+e^{y_{i}(w^{T}x_{i}+b)})^{2}}\\
\end{equation}

Then, we wish to show
\begin{equation*}
  \mathbf{a^THa} \equiv \sum_{j,k}a_ja_kH_{j,k} \geq 0
\end{equation*}

Note that summation (1) indicates the \(j,k^{th}\) element of the Hessian which allows us to rewrite the the above inequality as
\begin{align*}
  \sum_{j,k}a_ja_kH_{j,k} 
  &= \sum_{j,k}a_ja_k\sum_{i=1}^{N}x_{ij}x_{ik}\cdot\frac{e^{y_{i}(w^{T}x_{i}+b)}}{(1+e^{y_{i}(w^{T}x_{i}+b)})^{2}}\\
  &= \sum_{j,k}a_ja_k\sum_{i=1}^{N}x_{ij}x_{ik}\cdot\frac{e^{y_{i}(w^{T}x_{i}+b)}}{(1+e^{y_{i}(w^{T}x_{i}+b)})^{2}}\\
  &= \sum_{i=1}^{N}\frac{e^{y_{i}(w^{T}x_{i}+b)}}{(1+e^{y_{i}(w^{T}x_{i}+b)})^{2}}\sum_{j,k}a_ja_kx_{ij}x_{ik}\\
  &= \sum_{i=1}^{N}\frac{e^{y_{i}(w^{T}x_{i}+b)}}{(1+e^{y_{i}(w^{T}x_{i}+b)})^{2}}\sum_{j,k}\mathbf{a^Tx}a_kx_{ik}\\
  &= \sum_{i=1}^{N}\frac{e^{y_{i}(w^{T}x_{i}+b)}}{(1+e^{y_{i}(w^{T}x_{i}+b)})^{2}}\sum_{j,k}\mathbf{a^Tx}\mathbf{a^Tx}\\
  &= \sum_{i=1}^{N}\frac{e^{y_{i}(w^{T}x_{i}+b)}}{(1+e^{y_{i}(w^{T}x_{i}+b)})^{2}}\sum_{j,k}\mathbf{a^Tx}\mathbf{a^Tx}\\
  &= \sum_{i=1}^{N}\frac{e^{y_{i}(w^{T}x_{i}+b)}}{(1+e^{y_{i}(w^{T}x_{i}+b)})^{2}}\cdot(\mathbf{a^Tx})^2 \geq 0\\
\end{align*}
We show this summation is non-negative by showing each component of the summation is non-negative. Consider
\begin{align*}
  \sum_{i=1}^{N}\frac{\alpha}{\beta}\cdot\epsilon
  &= \sum_{i=1}^{N}\frac{e^{y_{i}(w^{T}x_{i}+b)}}{(1+e^{y_{i}(w^{T}x_{i}+b)})^{2}}\cdot(\mathbf{a^Tx})^2 \geq 0
\textnormal{Then, we realize that}\\
\alpha &= e^{y_{i}(w^{T}x_{i}+b)} > 0, \textnormal{since } e^z \textnormal{ is always positive}\\
\beta &= (1+e^{y_{i}(w^{T}x_{i}+b)})^{2} > 0\\
\epsilon &= (\mathbf{a^Tx})^2 \geq 0\\
\end{align*}

Therefore, \(L\) is convex. 
\end{document}
