\documentclass{article}
\usepackage{mathtools}
\usepackage{amssymb}
\begin{document}

Knowing 
\begin{equation*}
P(x) = \frac{1}{b}e^{-\frac{x}{b}}
\end{equation*}
(a)\\
We write the likelihood function given \(x_i\) as
\begin{align*}
\mathcal{L}(b|x_1,\hdots,x_N) 
&= \prod_{i = 1}^N \frac{1}{b}e^{-\frac{x}{b}}\\
&= \left(\frac{1}{b}\right)^N \prod_{i = 1}^N e^{-\frac{x}{b}}\\
&= \left(\frac{1}{b}\right)^N e^{\sum_{i=0}^N \frac{x_i}{b}}
\end{align*}
\\
(b)\\
We first find
\begin{align*}
log(\mathcal{L}) 
&= log\left(\left(\frac{1}{b}\right)^N e^{\sum_{i=0}^N \frac{x_i}{b}}\right)\\
&= log\left(\left(\frac{1}{b}\right)^N\right) + log\left(e^{\sum_{i=0}^N \frac{x_i}{b}}\right)\\
&= n(log(1) - log(b)) + \sum_{i=0}^N \frac{x_i}{b}log(e)
\end{align*}

Then,
\begin{align*}
\frac{\partial log \mathcal{L}}{\partial b}
&= \frac{\partial N(log(1) - log(b))}{\partial b} + \frac{\partial \sum_{i=0}^N \frac{x_i}{b}log(e)}{\partial b}\\
&= -\frac{N}{b} + \frac{\partial \frac{N}{b}\sum_{i=0}^N x_i\cdot log(e)}{\partial b}\\
&= -\frac{N}{b} - \frac{N}{b^2}\sum_{i=0}^N x_i\cdot log(e)\\
&= -\frac{N}{b}\left(1-\frac{1}{b}\sum_{i=0}^N x_i log(e)\right)
\end{align*}

(c)\\
We aim to maximize \(\mathcal{L}\) so,
\begin{equation*}
\frac{\partial \mathcal{L}}{\partial b} = -\frac{N}{b}\left(1-\frac{1}{b}\sum_{i=0}^N x_i log(e)\right) = 0
\end{equation*}
We can reassemble this as
\begin{align*}
-\frac{N}{b}\left(1-\frac{1}{b}log(e)\sum_{i=0}^N x_i\right)
&= 0\\
-N + \frac{N}{b}log(e)\sum_{i=0}^N x_i &= 0\\
\frac{N}{b}log(e)\sum_{i=0}^N x_i &= N\\
Nlog(e)\sum_{i=0}^N x_i &= Nb\\
log(e)\sum_{i=0}^N x_i &= b
\end{align*}

\end{document}
